setting up some lemma to prove a lower bound on edges of a connected graph

examples/data_structures/graph/Graph.Base.fst
@@ -1,26 +1,45 @@
 module Graph.Base
 
 module S = FStar.Seq
-module L = FStar.List
+module L = FStar.List.Tot
 open FStar.Fin
-
-let _in (s:S.seq 'a) = k:nat{k < S.length s}
+open Seq.Complements
 
 let graph0 (n:nat) = s:S.seq (list (fin n)){S.length s == n}
 
 let no_self_loop (#n:nat) (g:graph0 n) =
-  forall (i:_in g). not (L.mem (i <: fin n) (S.index g i))
+  forall (i:_in g). not (L.mem (i <: fin n) (g @^ i))
 
 let no_parallel_edge (#n:nat) (g:graph0 n) =
-  forall (i:_in g). L.noRepeats (S.index g i)
+  forall (i:_in g). L.noRepeats (g @^ i)
 
 let undirected (#n:nat) (g:graph0 n) =
-  forall (i:_in g) (k:fin n). L.mem k (S.index g i) ==> i < k
+  forall (i:_in g) (k:fin n). L.mem k (g @^ i) ==> i < k
 
-let graph (n:nat) = g:graph0 n{no_self_loop g /\ no_parallel_edge g /\ undirected g}
+let undirected_graph (n:nat) = g:graph0 n{no_self_loop g /\ no_parallel_edge g /\ undirected g}
 
 let node_size (#n:nat) (g:graph0 n) = S.length g
 
 let edge_size (#n:nat) (g:graph0 n) =
   L.fold_left (+) 0 (L.map L.length (S.seq_to_list g))
 
+let prepath (n:nat) = S.seq (fin n)
+
+let valid_path (#n:nat) (g:graph0 n) (p:prepath n) =
+  S.length p > 0 /\ (forall (i:nat{i < S.length p - 1}). L.mem (p @^ i+1) (g @^ p @^ i))
+
+let path (#n:nat) (g:graph0 n) = p:prepath n{valid_path #n g p}
+
+let from (#n:nat) (#g:graph0 n) (p:path g) = S.head p
+let to (#n:nat) (#g:graph0 n) (p:path g) = S.last p
+
+let empty_path_at (#n:nat) (g:graph0 n) (i:_in g) : path g =
+  S.create 1 i
+
+let elementary (#n:nat) (p:prepath n) = L.noRepeats (S.seq_to_list p)
+
+let length (#n:nat) (p:prepath n) = S.length p
+
+let prefix (#n:nat) (p1 p2:prepath n) = length p1 <= length p2 /\ (forall (i:_in p1). p1 @^ i == p2 @^ ((i <: nat) <: _in p2))
+
+let elementary_cycle (#n:nat) (#g:graph0 n) (p:path g) = elementary (S.slice p 1 (length p)) /\ from p == to p
