examples/data_structures/graph/Graph.Tree.fst
@@ -1,0 +1,57 @@
+module Graph.Tree
+
+open Graph.Base
+open Seq.Complements
+
+module S = FStar.Seq
+module L = FStar.List.Tot
+
+let connected (#n:nat) (g:graph0 n) =
+  forall (i j:_in g). exists (p:path g). from p == i /\ to p == j
+
+
+(* TODO : the basic structure of this lemma is set up but it still needs to be proven *)
+let rec extremal_node_or_cycle_from_aux (#n:nat) (g:graph0 n) (p:path g)
+  : Pure (either (_in g) (path g))
+    (requires (elementary p))
+    (ensures (fun r -> match r with | Inl i -> g @^ i == [] | Inr p' -> elementary_cycle p'))
+    (decreases (n - length p))
+= (* TODO : Remove me !!! *) admit () ;
+  match g @^ (to p) with
+  | [] -> Inl (to p)
+  | i :: _ ->
+    match S.seq_find (fun j -> j = i) p with
+    | None -> extremal_node_or_cycle_from_aux #n g (p `snoc` i)
+    | Some i0 ->
+      Inr (S.slice p i0 (length p) `snoc` i)
+
+let extremal_node_or_cycle_from
+  (#n:nat)
+  (g:graph0 n)
+  (i0:_in g)
+  : either (i:_in g{g @^ i == []}) (p:path g{elementary_cycle p})
+= match extremal_node_or_cycle_from_aux #n g (empty_path_at g i0) with
+  | Inl i -> Inl i
+  | Inr p -> Inr p
+
+
+let rec disconnected (#n:nat) (g:graph0 n)
+  : Lemma (requires (connected g /\ edge_size g < n - 1)) (ensures False)
+    (decreases (node_size g + edge_size g))
+= if edge_size g = 0 then
+    (* There is no path between (g @^ 0) and (g @^ 1) *)
+    admit ()
+  else
+    match extremal_node_or_cycle_from g 0 with
+    | Inl i ->
+      let g' : graph0 (n-1) =
+        (* Removing node i preserves connectedness *)
+        admit ()
+      in
+      disconnected g'
+   | Inr p ->
+     let g' : graph0 n =
+       (* Removing an edge in an elementary_cycle preserves connectedness *)
+       admit ()
+     in
+     disconnected g'
