examples/data_structures/graph/Seq.Complements.fst
@@ -1,0 +1,7 @@
+module Seq.Complements
+
+open FStar.Seq
+
+let _in (s:seq 'a) = k:nat{k < length s}
+let ( @^ ) (s:seq 'a) (i:_in s) : 'a = index s i
+let snoc (s:seq 'a) (x:'a) = s `append` (create 1 x)
